Add rough implementation of escapes

extraction/Interop.ml
@@ -1,7 +1,12 @@
 exception NotImplemented of string
 
-let line_terminators = '\n' :: '\r' :: []
 let all_chars = List.init 128 (Char.chr)
+let line_terminators = '\n' :: '\r' :: []
+let white_spaces = List.map (Char.chr) ( 11 :: 13 :: 14 :: [])
+let digits = '0' :: '1' :: '2' :: '3' :: '4' :: '5' :: '6' :: '7' :: '8' :: '9' :: []
+let ascii_word_characters = 
+  let str = "ABCDEFGHIJKLMNOPQRSTUVWXYZabcdefghijklmnopqrstuvwxyz0123456789_" in
+  List.init (String.length str) (String.get str)
 
 let code_point c = c
 let to_upper_case c = Char.uppercase_ascii c
