test/Tests.ml
@@ -4,28 +4,28 @@ open Warblre.Notations
 
 let%expect_test "char_class_atom_0_pos" =
   test_regex
-    (CharacterClass (NoninvertedCC (ClassAtomCR ('a', EmptyCR))))
+    (CharacterClass (NoninvertedCC (ClassAtomCR (SourceCharacter 'a', EmptyCR))))
     "abbb"
     0 ();
   [%expect {| Matched 1 characters ([0-1]) in 'abbb' (length=4) |}]
 
 let%expect_test "char_class_atom_0_neg" =
   test_regex
-    (CharacterClass (NoninvertedCC (ClassAtomCR ('b', EmptyCR))))
+    (CharacterClass (NoninvertedCC (ClassAtomCR (SourceCharacter 'b', EmptyCR))))
     "abbb"
     0 ();
   [%expect {| No match on 'abbb' |}]
 
 let%expect_test "negated_char_class_atom_0_pos" =
   test_regex
-    (CharacterClass (InvertedCC (ClassAtomCR ('b', EmptyCR))))
+    (CharacterClass (InvertedCC (ClassAtomCR (SourceCharacter 'b', EmptyCR))))
     "abbb"
     0 ();
   [%expect {| Matched 1 characters ([0-1]) in 'abbb' (length=4) |}]
 
 let%expect_test "negated_char_class_atom_0_neg" =
   test_regex
-    (CharacterClass (InvertedCC (ClassAtomCR ('a', EmptyCR))))
+    (CharacterClass (InvertedCC (ClassAtomCR (SourceCharacter 'a', EmptyCR))))
     "abbb"
     0 ();
   [%expect {| No match on 'abbb' |}]
@@ -35,35 +35,35 @@ let%expect_test "negated_char_class_atom_0_neg" =
 
 let%expect_test "char_class_seq_0_pos_0" =
   test_regex
-    (CharacterClass (NoninvertedCC (RangeCR ('a', 'c', EmptyCR))))
+    (CharacterClass (NoninvertedCC (RangeCR (SourceCharacter 'a', SourceCharacter 'c', EmptyCR))))
     "abbb"
     0 ();
   [%expect {| Matched 1 characters ([0-1]) in 'abbb' (length=4) |}]
 
 let%expect_test "char_class_seq_0_pos_1" =
   test_regex
-    (CharacterClass (NoninvertedCC (RangeCR ('a', 'c', EmptyCR))))
+    (CharacterClass (NoninvertedCC (RangeCR (SourceCharacter 'a', SourceCharacter 'c', EmptyCR))))
     "bbbb"
     0 ();
   [%expect {| Matched 1 characters ([0-1]) in 'bbbb' (length=4) |}]
 
 let%expect_test "char_class_seq_0_pos_2" =
   test_regex
-    (CharacterClass (NoninvertedCC (RangeCR ('a', 'c', EmptyCR))))
+    (CharacterClass (NoninvertedCC (RangeCR (SourceCharacter 'a', SourceCharacter 'c', EmptyCR))))
     "cbbb"
     0 ();
   [%expect {| Matched 1 characters ([0-1]) in 'cbbb' (length=4) |}]
 
 let%expect_test "char_class_seq_0_neg_0" =
   test_regex
-    (CharacterClass (NoninvertedCC (RangeCR ('a', 'c', EmptyCR))))
+    (CharacterClass (NoninvertedCC (RangeCR (SourceCharacter 'a', SourceCharacter 'c', EmptyCR))))
     " bbb"
     0 ();
   [%expect {| No match on ' bbb' |}]
 
 let%expect_test "char_class_seq_0_neg_1" =
   test_regex
-    (CharacterClass (NoninvertedCC (RangeCR ('a', 'c', EmptyCR))))
+    (CharacterClass (NoninvertedCC (RangeCR (SourceCharacter 'a', SourceCharacter 'c', EmptyCR))))
     "dbbb"
     0 ();
   [%expect {| No match on 'dbbb' |}]
@@ -74,35 +74,35 @@ let%expect_test "char_class_seq_0_neg_1" =
 
 let%expect_test "negated_char_class_seq_0_neg_0" =
   test_regex
-    (CharacterClass (InvertedCC (RangeCR ('a', 'c', EmptyCR))))
+    (CharacterClass (InvertedCC (RangeCR (SourceCharacter 'a', SourceCharacter 'c', EmptyCR))))
     "abbb"
     0 ();
   [%expect {| No match on 'abbb' |}]
 
 let%expect_test "negated_char_class_seq_0_neg_1" =
   test_regex
-    (CharacterClass (InvertedCC (RangeCR ('a', 'c', EmptyCR))))
+    (CharacterClass (InvertedCC (RangeCR (SourceCharacter 'a', SourceCharacter 'c', EmptyCR))))
     "bbbb"
     0 ();
   [%expect {| No match on 'bbbb' |}]
 
 let%expect_test "negated_char_class_seq_0_neg_2" =
   test_regex
-    (CharacterClass (InvertedCC (RangeCR ('a', 'c', EmptyCR))))
+    (CharacterClass (InvertedCC (RangeCR (SourceCharacter 'a', SourceCharacter 'c', EmptyCR))))
     "cbbb"
     0 ();
   [%expect {| No match on 'cbbb' |}]
 
 let%expect_test "negated_char_class_seq_0_pos_0" =
   test_regex
-    (CharacterClass (InvertedCC (RangeCR ('a', 'c', EmptyCR))))
+    (CharacterClass (InvertedCC (RangeCR (SourceCharacter 'a', SourceCharacter 'c', EmptyCR))))
     " bbb"
     0 ();
   [%expect {| Matched 1 characters ([0-1]) in ' bbb' (length=4) |}]
 
 let%expect_test "negated_char_class_seq_0_pos_1" =
   test_regex
-    (CharacterClass (InvertedCC (RangeCR ('a', 'c', EmptyCR))))
+    (CharacterClass (InvertedCC (RangeCR (SourceCharacter 'a', SourceCharacter 'c', EmptyCR))))
     "dbbb"
     0 ();
   [%expect {|Matched 1 characters ([0-1]) in 'dbbb' (length=4) |}]
@@ -340,28 +340,28 @@ let%expect_test "backref_long_neg_3" =
 
 let%expect_test "case_insensitive_0_pos_0" =
   test_regex
-    (CharacterClass (NoninvertedCC (ClassAtomCR ('a', EmptyCR))))
+    (CharacterClass (NoninvertedCC (ClassAtomCR (SourceCharacter 'a', EmptyCR))))
     "abbb"
     0 ~ignoreCase:true ();
   [%expect {| Matched 1 characters ([0-1]) in 'abbb' (length=4) |}]
 
 let%expect_test "case_insensitive_0_pos_1" =
   test_regex
-    (CharacterClass (NoninvertedCC (ClassAtomCR ('a', EmptyCR))))
+    (CharacterClass (NoninvertedCC (ClassAtomCR (SourceCharacter 'a', EmptyCR))))
     "Abbb"
     0 ~ignoreCase:true ();
   [%expect {| Matched 1 characters ([0-1]) in 'Abbb' (length=4) |}]
 
 let%expect_test "case_insensitive_0_pos_2" =
   test_regex
-    (CharacterClass (NoninvertedCC (ClassAtomCR ('A', EmptyCR))))
+    (CharacterClass (NoninvertedCC (ClassAtomCR (SourceCharacter 'A', EmptyCR))))
     "abbb"
     0 ~ignoreCase:true ();
   [%expect {| Matched 1 characters ([0-1]) in 'abbb' (length=4) |}]
 
 let%expect_test "case_insensitive_0_pos_3" =
   test_regex
-    (CharacterClass (NoninvertedCC (ClassAtomCR ('A', EmptyCR))))
+    (CharacterClass (NoninvertedCC (ClassAtomCR (SourceCharacter 'A', EmptyCR))))
     "Abbb"
     0 ~ignoreCase:true ();
   [%expect {| Matched 1 characters ([0-1]) in 'Abbb' (length=4) |}]
@@ -369,14 +369,14 @@ let%expect_test "case_insensitive_0_pos_3" =
 
 let%expect_test "case_insensitive_0_neg_0" =
   test_regex
-    (CharacterClass (NoninvertedCC (ClassAtomCR ('a', EmptyCR))))
+    (CharacterClass (NoninvertedCC (ClassAtomCR (SourceCharacter 'a', EmptyCR))))
     "bbbb"
     0 ~ignoreCase:true ();
   [%expect {| No match on 'bbbb' |}]
 
 let%expect_test "case_insensitive_0_neg_1" =
   test_regex
-    (CharacterClass (NoninvertedCC (ClassAtomCR ('a', EmptyCR))))
+    (CharacterClass (NoninvertedCC (ClassAtomCR (SourceCharacter 'a', EmptyCR))))
     "Bbbb"
     0 ~ignoreCase:true ();
   [%expect {| No match on 'Bbbb' |}]
